Splinter/Betree/BranchedBetreeRefinement.i.dfy
@@ -1,0 +1,315 @@
+// Copyright 2018-2021 VMware, Inc., Microsoft Inc., Carnegie Mellon University, ETH Zurich, and University of Washington
+// SPDX-License-Identifier: BSD-2-Clause
+
+include "LinkedBetree.i.dfy"
+include "BranchedBetree.i.dfy"
+
+module BranchedBetreeRefinement {
+  import opened BoundedPivotsLib
+  import LinkedBetree = LinkedBetreeMod
+  import opened BranchedBetreeMod
+  import opened LinkedBranchMod
+  import opened BranchesMod
+  import opened StampedMod
+  import opened DomainMod
+  import opened Buffers
+  import opened KeyType
+  import opened Sequences
+
+  import opened ValueMessage // test
+
+  function ILbl(lbl: TransitionLabel) : LinkedBetree.TransitionLabel
+  {
+    match lbl
+      case QueryLabel(endLsn, key, value) => LinkedBetree.QueryLabel(endLsn, key, value)
+      case PutLabel(puts) => LinkedBetree.PutLabel(puts)
+      case QueryEndLsnLabel(endLsn) => LinkedBetree.QueryEndLsnLabel(endLsn)
+      case FreezeAsLabel(stampedBetree) => LinkedBetree.FreezeAsLabel(
+        if stampedBetree.value.WF() && stampedBetree.value.Valid()
+        then IStampedBetree(stampedBetree)
+        else IStampedBetree(EmptyImage())  // "silly" case, since we never interpret non-(WF+Valid) things
+      )
+      case InternalAllocationsLabel(treeAddrs, _) => LinkedBetree.InternalAllocationsLabel(treeAddrs)
+      case InternalLabel() => LinkedBetree.InternalLabel()
+  }
+
+  function ActiveBufferKeysForChild(node: BetreeNode, childIdx: nat, bufferIdx: nat) : iset<Key>
+    requires node.WF()
+    requires childIdx < |node.children|
+    requires bufferIdx < |node.buffers|
+  {
+    if node.activeBufferRanges[childIdx] <= bufferIdx 
+    then node.DomainRoutedToChild(childIdx).KeySet()
+    else iset{}
+  }
+
+  function ActiveBufferKeys(node: BetreeNode, bufferIdx: nat) : iset<Key>
+    requires node.WF()
+    requires bufferIdx < |node.buffers|
+  {
+    iset k, i | 0 <= i < |node.children| && k in ActiveBufferKeysForChild(node, i, bufferIdx) :: k
+  }
+
+  function IBuffer(node: BetreeNode, branch: LinkedBranch, bufferIdx: nat) : Buffer
+    requires node.WF()
+    requires bufferIdx < |node.buffers|
+    requires branch.Acyclic()
+    requires branch.AllKeysInRange()
+  {
+    var buffer := branch.I().I();
+    buffer.ApplyFilter(ActiveBufferKeys(node, bufferIdx))
+  }
+
+  function IBufferStack(node: BetreeNode, branches: Branches) : BufferStack
+    requires node.WF()
+    requires branches.WF()
+    requires forall buffer | buffer in node.buffers :: branches.ValidBranch(buffer)
+  {
+    BufferStack( seq (|node.buffers|, 
+         i requires 0 <= i < |node.buffers| => 
+         IBuffer(node, branches.GetBranch(node.buffers[i]), i)))
+  }
+
+  function IBranchedBetreeNode(node: BetreeNode, branches: Branches) : (out: LinkedBetree.BetreeNode)
+    requires node.WF()
+    requires branches.WF()
+    requires forall buffer | buffer in node.buffers :: branches.ValidBranch(buffer)
+    ensures out.WF()
+  {
+    LinkedBetree.BetreeNode(IBufferStack(node, branches), node.pivotTable, node.children)
+  }
+
+  function IDiskView(branched: BranchedBetree) : (out: LinkedBetree.DiskView)
+    requires branched.WF()
+    requires branched.Valid()
+    ensures out.WF()
+  {
+    var entries := branched.diskView.entries;
+    var dv := LinkedBetree.DiskView( map addr | addr in entries ::
+                IBranchedBetreeNode(entries[addr], branched.branches));
+
+    assert dv.HealthyChildPointers(); // trigger
+    dv
+  }
+
+  function IBranchedBetree(branched: BranchedBetree) : (out: LinkedBetree.LinkedBetree)
+    requires branched.WF()
+    requires branched.Valid()
+    ensures out.WF()
+  {
+    LinkedBetree.LinkedBetree(branched.root, IDiskView(branched))
+  }
+
+  function IStampedBetree(stampedBetree: StampedBetree) : (out: LinkedBetree.StampedBetree)
+    requires stampedBetree.value.WF()
+    requires stampedBetree.value.Valid()
+    ensures out.value.WF()
+  {
+    Stamped(IBranchedBetree(stampedBetree.value), stampedBetree.seqEnd)
+  }
+
+  // Acyclic implies Acyclic
+  lemma IBranchedBetreeAcyclic(branched: BranchedBetree) 
+    requires branched.Acyclic()
+    requires branched.Valid()
+    ensures IBranchedBetree(branched).Acyclic()
+  {
+    assume false;
+  }
+
+  // Interpretation functions for Path
+  function IPath(path: Path) : LinkedBetree.Path
+    requires path.Valid()
+  {
+    LinkedBetree.Path(IBranchedBetree(path.branched), path.key, path.depth) 
+  }
+
+  // Interpretation functions for Query receipts
+  function IReceiptLine(line: QueryReceiptLine) : (out: LinkedBetree.QueryReceiptLine)
+    requires line.branched.WF()
+    requires line.branched.Valid()
+  {
+    LinkedBetree.QueryReceiptLine(IBranchedBetree(line.branched), line.result)
+  }
+
+   function IReceipt(receipt: QueryReceipt) : (out: LinkedBetree.QueryReceipt)
+    requires receipt.Valid()
+  {
+    LinkedBetree.QueryReceipt(
+      receipt.key, 
+      IBranchedBetree(receipt.branched), 
+      seq(|receipt.lines|, i requires 0<=i<|receipt.lines| => IReceiptLine(receipt.lines[i])))
+  }
+
+  lemma ActiveBuffersForKeyConsistent(node: BetreeNode, key: Key, start: nat)
+    requires node.WF()
+    requires node.KeyInDomain(key)
+    requires start == node.ActiveBuffersForKey(key)
+    ensures forall i:nat | i < start :: key !in ActiveBufferKeys(node, i)
+    ensures forall i:nat | start <= i < |node.buffers| :: key in ActiveBufferKeys(node, i)
+  {
+    forall i:nat | start <= i < |node.buffers|
+      ensures key in ActiveBufferKeys(node, i)
+    {
+      var childIdx := Route(node.pivotTable, key);
+      assert key in ActiveBufferKeysForChild(node, childIdx, i); // trigger
+    }
+  }
+
+  function BranchesBufferStack(branches: Branches, buffers: seq<Address>) : BufferStack
+    requires branches.WF()
+    requires (forall addr | addr in buffers :: branches.ValidBranch(addr))
+  {
+    BufferStack(seq (|buffers|, i requires 0 <= i < |buffers| => branches.GetBranch(buffers[i]).I().I()))
+  }
+
+  lemma BranchesBufferStackQueryConsistent(key: Key, branches: Branches, buffers: seq<Address>, count: nat)
+    requires count <= |buffers|
+    requires BranchesBufferStack.requires(branches, buffers)
+    ensures BranchesBufferStack(branches, buffers).QueryUpTo(key, count) == branches.Query(key, buffers[..count])
+  {
+    if count > 0 {
+      var bufferstack := BranchesBufferStack(branches, buffers);
+      var branch := branches.GetBranch(buffers[count-1]);
+      var msg := if branch.Query(key).Some? then branch.Query(key).value else Update(NopDelta());
+
+      assert bufferstack.buffers[count-1].Query(key) == msg;
+      assert buffers[..count-1] == DropLast(buffers[..count]);
+
+      BranchesBufferStackQueryConsistent(key, branches, buffers, count-1);
+    }
+  }
+
+  lemma IReceiptValid(receipt: QueryReceipt) 
+    requires receipt.Valid()
+    ensures IReceipt(receipt).Valid()
+  {
+    var ireceipt := IReceipt(receipt);
+    var key := receipt.key;
+
+    IBranchedBetreeAcyclic(receipt.branched);
+
+    forall i:nat | i < |ireceipt.lines|
+      ensures ireceipt.lines[i].linked.Acyclic()
+    {
+      IBranchedBetreeAcyclic(receipt.lines[i].branched);
+    }
+
+    forall i:nat | i < |ireceipt.lines|-1 
+      ensures ireceipt.Node(i).KeyInDomain(key)
+      ensures ireceipt.ChildLinkedAt(i)
+    {
+      assert receipt.Node(i).KeyInDomain(key);  // trigger
+      assert receipt.ChildLinkedAt(i);  // trigger
+    }
+  
+    forall i:nat | i < |ireceipt.lines| - 1 
+    ensures ireceipt.ResultLinkedAt(i)
+    {
+      assert receipt.ResultLinkedAt(i);  // trigger
+      
+      var key := ireceipt.key;
+      var branched := receipt.lines[i].branched;
+      var linked := ireceipt.lines[i].linked;
+
+      var node := branched.Root();
+      var start := node.ActiveBuffersForKey(key);
+      var activeBuffers := node.buffers[start..];
+      var activeBufferStack := BranchesBufferStack(branched.branches, activeBuffers);
+
+      assert activeBuffers[..|activeBuffers|] == activeBuffers;
+      BranchesBufferStackQueryConsistent(key, branched.branches, activeBuffers, |activeBuffers|);
+      assert activeBufferStack.Query(key) == branched.branches.Query(key, activeBuffers);
+
+      var buffers := linked.Root().buffers;
+      ActiveBuffersForKeyConsistent(node, key, start);
+
+      var right := buffers.SliceRight(start);
+      right.QueryUpToEquivalent(key, activeBufferStack, |right.buffers|);
+      buffers.QueryEmptyLeft(key, start, |buffers.buffers|);
+
+      assert ireceipt.ResultLinkedAt(i);  // trigger
+    }
+  }
+
+  // Interpretation functions for Steps
+  function IStepDefn(step: Step) : (out: LinkedBetree.Step)
+    requires step.WF()
+  {
+    match step {
+      case QueryStep(receipt) => LinkedBetree.QueryStep(IReceipt(receipt))
+      case PutStep() => LinkedBetree.PutStep()
+      case QueryEndLsnStep() => LinkedBetree.QueryEndLsnStep()
+      case FreezeAsStep() => LinkedBetree.FreezeAsStep()
+      case InternalGrowStep(newRootAddr) => LinkedBetree.InternalGrowStep(newRootAddr)
+      case InternalSplitStep(path, request, newAddrs, pathAddrs) => 
+            LinkedBetree.InternalSplitStep(IPath(path), request, newAddrs, pathAddrs)
+      case InternalFlushMemtableStep(newRootAddr, _) => LinkedBetree.InternalFlushMemtableStep(newRootAddr)
+      case InternalFlushStep(path, childIdx, targetAddr, targetChildAddr, pathAddrs, _) =>
+            LinkedBetree.InternalFlushStep(IPath(path), childIdx, targetAddr, targetChildAddr, pathAddrs)
+      case InternalCompactStep(path, compactStart, compactEnd, _, targetAddr, pathAddrs) => (
+          var linked := IBranchedBetree(path.Target());
+          var compactedBuffers := linked.Root().buffers.buffers[compactStart..compactEnd];
+          LinkedBetree.InternalCompactStep(IPath(path), BufferStack(compactedBuffers), targetAddr, pathAddrs))
+      case InternalPruneBranchesStep(_) => LinkedBetree.InternalNoOpStep()
+      case InternalNoOpStep() => LinkedBetree.InternalNoOpStep()
+    }
+  }
+
+  lemma IStepWF(step: Step)
+    requires IStepDefn.requires(step)
+    ensures IStepDefn(step).WF()
+  {
+    var istep := IStepDefn(step);
+    match step {
+      case QueryStep(receipt) => { IReceiptValid(receipt); }
+      case InternalSplitStep(path, request, newAddrs, pathAddrs) => {
+      //   IPathValid(step.path);
+      //   TargetCommutesWithI(step.path);
+
+      //   assert istep.path.Target().CanSplitParent(istep.request) by {
+      //     var target := step.path.Target();
+      //     var ichild := istep.path.Target().children[request.childIdx];
+      //     var child := target.ChildAtIdx(request.childIdx);
+      //     assert ILinkedBetreeNode(target, target.TheRanking()).children[request.childIdx]
+      //       == ILinkedBetreeNode(child, target.TheRanking());  // trigger
+      //     assert ichild.children[0] == IChildren(child, target.TheRanking())[0];  // trigger
+
+      //     if step.request.SplitLeaf? {
+      //       assert IChildren(child, target.TheRanking())[0] == PivotBetree.Nil;  // trigger
+      //     } else {
+      //       forall i | 0 <= i < |ichild.children| ensures ichild.children[i].BetreeNode? {
+      //         assert ichild.children[i] == ILinkedBetreeNode(child.ChildAtIdx(i), target.TheRanking()); // trigger
+      //       }
+      //     }
+      //   }
+        // assert istep.WF();  // case boilerplate
+        assume false;
+      }
+      case InternalFlushStep(path, childIdx, _, _, _, _) => {
+      //   IPathValid(step.path);
+      //   TargetCommutesWithI(step.path);
+      //   assert istep.WF();  // case boilerplate
+        assume false;
+      }
+      // case InternalFlushMemtableStep(_, _) => { assert istep.WF(); }
+      case InternalCompactStep(path, compactedBuffers, _, _, _, _) => {
+      //   IPathValid(step.path);
+      //   TargetCommutesWithI(step.path);
+      //   assert istep.WF();  // case boilerplate
+        assume false;
+      }
+      case _ =>    {  assert istep.WF(); }
+    }
+  }
+
+  function IStep(step: Step) : (out: LinkedBetree.Step)
+    requires step.WF()
+    ensures out.WF()
+  {
+    IStepWF(step);
+    IStepDefn(step)
+  }
+
+
+}
