Splinter/Betree/Branches.i.dfy
@@ -1,0 +1,71 @@
+// Copyright 2018-2021 VMware, Inc., Microsoft Inc., Carnegie Mellon University, ETH Zurich, and University of Washington
+// SPDX-License-Identifier: BSD-2-Clause
+
+include "../Journal/GenericDisk.i.dfy"
+include "LinkedBranch.i.dfy"
+
+module BranchesMod {
+	import opened KeyType
+	import opened ValueMessage
+  import opened Maps
+	import opened Sequences
+	import opened LinkedBranchMod
+  import D = GenericDisk
+
+  function EmptyBranches() : Branches
+  {
+    Branches({}, DiskView.DiskView(map[]))
+  }
+
+	// Track the branches as branchroot and a single diskView
+	// We can construct LinkedBranch from each tree and the diskView
+	datatype Branches = Branches(roots: set<Address>, diskView: DiskView) 
+	{
+		predicate WF() {
+			&& diskView.WF() // ensures all nodes are connected
+			&& (forall root | root in roots :: diskView.ValidAddress(root))
+      && (forall root | root in roots :: GetBranch(root).Acyclic())
+      && (forall root | root in roots :: GetBranch(root).AllKeysInRange())
+		}
+
+		predicate ValidBranch(addr: Address)
+		{
+			addr in roots
+		}
+
+		function GetBranch(addr: Address) : (branch: LinkedBranch)
+      requires ValidBranch(addr)
+		{
+			LinkedBranch(addr, diskView)
+		}
+
+		function Query(key: Key, buffers: seq<Address>) : Message
+      requires WF()
+      requires (forall addr | addr in buffers :: ValidBranch(addr))
+		{
+			if buffers == [] then Update(NopDelta())
+      else (
+				var branch := GetBranch(Last(buffers));
+        var msg := if branch.Query(key).Some? then branch.Query(key).value else Update(NopDelta());
+				Merge(Query(key, DropLast(buffers)), msg)
+			)
+		}
+
+    function AddBranch(branch: LinkedBranch) : Branches
+      requires WF()
+      requires branch.Acyclic()
+      requires branch.TightDiskView()
+      requires diskView.IsFresh(branch.ReachableAddrs())
+    {
+      Branches(roots + {branch.root}, diskView.MergeDisk(branch.diskView))
+    }
+    
+    function RemoveBranch(root: Address) : Branches
+      requires WF()
+      requires ValidBranch(root)
+    {
+      var branchDisk := DiskView(MapRestrict(diskView.entries, GetBranch(root).ReachableAddrs()));
+      Branches(roots - {root}, diskView.RemoveDisk(branchDisk))
+    }
+	}
+}
