Splinter/Betree/PivotBranch.i.dfy
@@ -182,32 +182,59 @@ module PivotBranchMod {
         result
       )
     }
-  
+
+    // filter = keys to remove
     predicate IsFiltered(og: Node, filter: Domain)
       requires WF()
       requires og.WF()
       requires !filter.EmptyDomain?
     {
-      && (forall k :: Query(k).Some? <==> (filter.Contains(k) && og.Query(k).Some?))  // define this's domain
+      && (forall k :: Query(k).Some? <==> (!filter.Contains(k) && og.Query(k).Some?))  // define this's domain
       && (forall k | Query(k).Some? :: Query(k) == og.Query(k)) // value matches og
     }
 
     lemma FilteredEquivApplyFilter(og: Node, filter: Domain)
       requires IsFiltered.requires(og, filter)
       requires IsFiltered(og, filter)
-      ensures I() == og.I().ApplyFilter(filter.KeySet())
+      ensures I() == og.I().ApplyFilter(Buffers.AllKeys() - filter.KeySet())
     {
       var actual := I();
-      var expected := og.I().ApplyFilter(filter.KeySet());
+      var expected := og.I().ApplyFilter(Buffers.AllKeys() - filter.KeySet());
 
-      assert (forall k :: k in actual.mapp <==> (filter.Contains(k) && og.Query(k).Some?));
-      assert (forall k :: k in expected.mapp <==> (filter.Contains(k) && og.Query(k).Some?));
+      assert (forall k :: k in actual.mapp <==> (!filter.Contains(k) && og.Query(k).Some?));
+      assert (forall k :: k in expected.mapp <==> (!filter.Contains(k) && og.Query(k).Some?));
       assert (forall k :: k in actual.mapp <==> k in expected.mapp);
 
       assert IsSubMap(actual.mapp, expected.mapp);
       assert IsSubMap(expected.mapp, actual.mapp);
       MapEquality(actual.mapp, expected.mapp);
     }
+  
+    // predicate IsFiltered(og: Node, filter: Domain)
+    //   requires WF()
+    //   requires og.WF()
+    //   requires !filter.EmptyDomain?
+    // {
+    //   && (forall k :: Query(k).Some? <==> (filter.Contains(k) && og.Query(k).Some?))  // define this's domain
+    //   && (forall k | Query(k).Some? :: Query(k) == og.Query(k)) // value matches og
+    // }
+
+    // lemma FilteredEquivApplyFilter(og: Node, filter: Domain)
+    //   requires IsFiltered.requires(og, filter)
+    //   requires IsFiltered(og, filter)
+    //   ensures I() == og.I().ApplyFilter(filter.KeySet())
+    // {
+    //   var actual := I();
+    //   var expected := og.I().ApplyFilter(filter.KeySet());
+
+    //   assert (forall k :: k in actual.mapp <==> (filter.Contains(k) && og.Query(k).Some?));
+    //   assert (forall k :: k in expected.mapp <==> (filter.Contains(k) && og.Query(k).Some?));
+    //   assert (forall k :: k in actual.mapp <==> k in expected.mapp);
+
+    //   assert IsSubMap(actual.mapp, expected.mapp);
+    //   assert IsSubMap(expected.mapp, actual.mapp);
+    //   MapEquality(actual.mapp, expected.mapp);
+    // }
 
     // Note: intended for iterator which we currently don't have
     function Flatten() : (result: FlattenedBranch)
